coq/TypedSyntax.v
@@ -60,73 +60,122 @@ Section Syntax.
     | CtxCons k v ctx => P k v /\ ctx_Forall P ctx
     end.
 
-  Lemma action_ind_complete :
-    forall P : forall (sig : tsig var_t) (tau : type), action sig tau -> Prop,
+  Definition acontext (sig argspec: tsig var_t) :=
+    context (fun k_tau => action sig (snd k_tau)) argspec.
 
+  (* This induction principle contains all necessary
+    hypothesis to do an actual induction over an `action`
+    without resorting to manual Fixpoint proofs.
+
+    Note that this principle can only be used on goals
+    of the form `Pa /\ Pargs` where `Pa` stand for an arbitrary
+    proposition over actions while `Pargs` represents an
+    analogus porp extended to contexts of actions (just
+      like they are used by `InternalCall`)
+
+    As an example, have a look at the proofs in Hoare.v
+  *)
+  Lemma action_ind_complete :
+    (* Propositions *)
+    forall P : forall {sig tau}, action sig tau -> Prop,
+    forall P' : forall {sig argspec}, acontext sig argspec -> Prop,
+
+    (* All cases for the normal action *)
     (forall (sig : tsig var_t) (tau : type),
-      P sig tau (Fail tau)) ->
+      @P sig tau (Fail tau)) ->
     (forall (sig : list (var_t * type)) (k : var_t) (tau : type) (m : member (k, tau) sig),
-      P sig tau (Var m)) ->
+      @P sig tau (Var m)) ->
     (forall (sig : tsig var_t) (tau : type) (cst : tau),
-      P sig tau (Const cst)) ->
+      @P sig tau (Const cst)) ->
     (forall (sig : list (var_t * type)) (k : var_t) (tau : type) (m : member (k, tau) sig) (ex : action sig tau),
-      P sig tau ex ->
-      P sig unit_t (Assign m ex)) ->
+      @P sig tau ex ->
+      @P sig unit_t (Assign m ex)) ->
     (forall (sig : tsig var_t) (tau : type) (r1 : action sig unit_t) (r2 : action sig tau),
-      P sig unit_t r1 ->
-      P sig tau r2 ->
-      P sig tau (Seq r1 r2)) ->
+      @P sig unit_t r1 ->
+      @P sig tau r2 ->
+      @P sig tau (Seq r1 r2)) ->
     (forall (sig : tsig var_t) (tau tau' : type) (var : var_t) (ex : action sig tau) (body : action ((var, tau) :: sig) tau'),
-      P sig tau ex ->
-      P ((var, tau) :: sig) tau' body ->
-      P sig tau' (Bind var ex body)) ->
+      @P sig tau ex ->
+      @P ((var, tau) :: sig) tau' body ->
+      @P sig tau' (Bind var ex body)) ->
     (forall (sig : tsig var_t) (tau : type) (cond : action sig (bits_t 1)) (tbranch : action sig tau) (fbranch : action sig tau),
-      P sig (bits_t 1) cond ->
-      P sig tau tbranch ->
-      P sig tau fbranch ->
-      P sig tau (If cond tbranch fbranch)) ->
+      @P sig (bits_t 1) cond ->
+      @P sig tau tbranch ->
+      @P sig tau fbranch ->
+      @P sig tau (If cond tbranch fbranch)) ->
     (forall (sig : tsig var_t) (port : Port) (idx : reg_t),
-      P sig (R idx) (Read port idx)) ->
+      @P sig (R idx) (Read port idx)) ->
     (forall (sig : tsig var_t) (port : Port) (idx : reg_t) (value : action sig (R idx)),
-      P sig (R idx) value -> P sig unit_t (Write port idx value)) ->
+      @P sig (R idx) value ->
+      @P sig unit_t (Write port idx value)) ->
     (forall (sig : tsig var_t) (fn : fn1) (arg1 : action sig (arg1Sig (Sigma1 fn))),
-      P sig (arg1Sig (Sigma1 fn)) arg1 ->
-      P sig (retSig (Sigma1 fn)) (Unop fn arg1)) ->
+      @P sig (arg1Sig (Sigma1 fn)) arg1 ->
+      @P sig (retSig (Sigma1 fn)) (Unop fn arg1)) ->
     (forall (sig : tsig var_t) (fn : fn2) (arg1 : action sig (arg1Sig (Sigma2 fn))) (arg2 : action sig (arg2Sig (Sigma2 fn))),
-      P sig (arg1Sig (Sigma2 fn)) arg1 ->
-      P sig (arg2Sig (Sigma2 fn)) arg2 ->
-      P sig (retSig (Sigma2 fn)) (Binop fn arg1 arg2)) ->
+      @P sig (arg1Sig (Sigma2 fn)) arg1 ->
+      @P sig (arg2Sig (Sigma2 fn)) arg2 ->
+      @P sig (retSig (Sigma2 fn)) (Binop fn arg1 arg2)) ->
     (forall (sig : tsig var_t) (fn : ext_fn_t) (arg : action sig (arg1Sig (Sigma fn))),
-      P sig (arg1Sig (Sigma fn)) arg ->
-      P sig (retSig (Sigma fn)) (ExternalCall fn arg)) ->
+      @P sig (arg1Sig (Sigma fn)) arg ->
+      @P sig (retSig (Sigma fn)) (ExternalCall fn arg)) ->
     (forall (sig : tsig var_t) (tau : type) (argspec : tsig var_t) (fn : InternalFunction' fn_name_t (action argspec tau)) (args : context (fun k_tau : var_t * type => action sig (snd k_tau)) argspec),
-      P argspec tau fn.(int_body) ->
-      ctx_Forall (fun k_tau => P sig (snd k_tau)) args ->
-      P sig tau (InternalCall fn args)) ->
+      @P argspec tau fn.(int_body) ->
+      @P' sig argspec args ->
+      @P sig tau (InternalCall fn args)) ->
     (forall (sig : tsig var_t) (tau : type) (pos : pos_t) (a : action sig tau),
-      P sig tau a -> P sig tau (APos pos a)) ->
-    forall (sig : tsig var_t) (tau : type) (a : action sig tau), P sig tau a.
+      @P sig tau a ->
+      @P sig tau (APos pos a)) ->
+
+    (* All cases for action contexts *)
+    (forall sig,
+      @P' sig [] CtxEmpty) ->
+    (forall sig n tau argspec a args,
+      @P sig tau a ->
+      @P' sig argspec args ->
+      @P' sig ((n,tau) :: argspec) (CtxCons (n,tau) a args)) ->
+
+    (* goal *)
+    (forall {sig tau} (a : action sig tau),
+    @P sig tau a) /\
+    (forall {sig argspec} (args : acontext sig argspec),
+    @P' sig argspec args).
   Proof.
-    intros P H1 H2 H3 H4 H5 H6 H7 H8 H9 H10 H11 H12 H13 H14.
-    fix IH 3.
-    destruct a.
-    - apply H1.
-    - apply H2.
-    - apply H3.
-    - apply H4. auto.
-    - apply H5; auto.
-    - apply H6; auto.
-    - apply H7; auto.
-    - apply H8.
-    - apply H9. auto.
-    - apply H10. auto.
-    - apply H11; auto.
-    - apply H12. auto.
-    - apply H13. auto. clear fn.
-      induction args.
-      + cbn. auto.
-      + split. auto. assumption.
-    - apply H14. auto.
+    intros P P' H1 H2 H3 H4 H5 H6 H7 H8 H9 H10 H11 H12 H13 H14 H1' H2'.
+    assert (H : forall (sig : tsig var_t) (tau : type) (a : action sig tau), P sig tau a).
+    - fix IH 3.
+      destruct a.
+      + apply H1.
+      + apply H2.
+      + apply H3.
+      + apply H4; apply IH.
+      + apply H5; apply IH.
+      + apply H6; apply IH.
+      + apply H7; apply IH.
+      + apply H8.
+      + apply H9. apply IH.
+      + apply H10. apply IH.
+      + apply H11; apply IH.
+      + apply H12. apply IH.
+      + apply H13. apply IH.
+        clear fn.
+        revert sig argspec args.
+        fix IH' 3.
+        destruct args.
+        * apply H1'.
+        * destruct k.
+          apply H2'.
+          -- apply IH.
+          -- apply IH'.
+      + apply H14. apply IH.
+    - split.
+      + exact H.
+      + fix IH' 3.
+        destruct args.
+        apply H1'.
+        destruct k.
+        apply H2'.
+        -- apply H.
+        -- apply IH'.
   Qed.
 
   Definition rule := action nil unit_t.
